common/Memstructure.v
@@ -1,0 +1,140 @@
+Require Import Coqlib.
+Require Intv.
+Require Import Maps.
+Require Archi.
+Require Import AST.
+Require Import Integers.
+Require Import Floats.
+Require Import Values.
+Require Export Memdata.
+Require Export Memtype.
+Require Export Memory.
+(* To avoid useless definitions of inductors in extracted code. *)
+Local Unset Elimination Schemes.
+Local Unset Case Analysis Schemes.
+
+(* Module Type SUP(Block:BLOCK).
+Include Block.
+Parameter sup: Type.
+
+Parameter sup_empty : sup.
+
+Parameter sup_In : block -> sup -> Prop.
+Parameter empty_in: forall b, ~ sup_In b sup_empty.
+Parameter sup_dec : forall b s, {sup_In b s}+{~sup_In b s}.
+
+Parameter fresh_block : sup -> block.
+Parameter freshness : forall s, ~sup_In (fresh_block s) s.
+
+Parameter sup_add : block -> sup -> sup.
+
+Definition sup_incr(s:sup) := sup_add (fresh_block s) s.
+
+Definition sup_include(s1 s2:sup) := forall b, sup_In b s1 -> sup_In b s2.
+
+Parameter sup_add_in : forall b s b', sup_In b' (sup_add b s) <-> b' = b \/ sup_In b' s.
+
+Theorem sup_add_in1 : forall b s, sup_In b (sup_add b s).
+Proof. intros. apply sup_add_in. left. auto. Qed.
+Theorem sup_add_in2 : forall b s, sup_include s (sup_add b s).
+Proof. intros. intro. intro. apply sup_add_in. right. auto. Qed.
+
+Lemma sup_include_refl : forall s:sup, sup_include s s.
+Proof. intro. intro. auto. Qed.
+
+Lemma sup_include_trans:
+  forall p q r:sup,sup_include p q-> sup_include q r -> sup_include p r.
+Proof.
+  intros. intro. intro.  auto.
+Qed.
+
+Lemma sup_include_incr:
+  forall s b, sup_include s (sup_add b s).
+Proof.
+  intros. apply sup_add_in2.
+Qed.
+
+End SUP.*)
+
+Module Memstructure1.
+
+Module Block <: BLOCK.
+Inductive block' :=
+|Global : ident -> block'
+|Heap : ident -> block'
+|Stack : ident -> block'.
+
+Definition block := block'.
+Theorem eq_block : forall (x y:block),{x=y}+{x<>y}.
+Proof.
+  intros. destruct x; destruct y.
+  destruct (peq i i0). left; congruence. right; congruence.
+  right. congruence. right. congruence.
+  right. congruence.
+  destruct (peq i i0). left; congruence. right; congruence.
+  right. congruence.
+  right. congruence. right. congruence.
+  destruct (peq i i0). left; congruence. right; congruence.
+Qed.
+End Block.
+
+Module Mem := Mem(Block).
+Include Block.
+
+Record structure := mk_struc{
+ global_sup: list ident;
+ heap_sup: list ident;
+ stack_sup: list ident;
+}.
+
+Definition structure_In (b:block)(s:structure) :=
+  match b with
+    |Global id => In id (global_sup s)
+    |Heap id => In id (heap_sup s)
+    |Stack id => In id (stack_sup s)
+  end.
+
+
+Definition match_mem_structure (m:Mem.mem) (s:structure) :=
+   forall b, Mem.valid_block m b <-> structure_In b s.
+
+Fixpoint find_max_pos (l: list positive) : positive :=
+  match l with
+  |nil => 1
+  |hd::tl => let m' := find_max_pos tl in
+             match plt hd m' with
+             |left _ => m'
+             |right _ => hd
+             end
+  end.
+
+Theorem Lessthan: forall p l, In p l -> Ple p (find_max_pos l).
+Proof.
+  intros.
+  induction l.
+  destruct H.
+  destruct H;simpl.
+  - destruct (plt a (find_max_pos l)); subst a.
+    + apply Plt_Ple. assumption.
+    + apply Ple_refl.
+  - destruct (plt a (find_max_pos l)); apply IHl in H.
+    + auto.
+    + eapply Ple_trans. eauto.  apply Pos.le_nlt. apply n.
+Qed.
+
+Definition fresh_ident (l: list ident ) := Pos.succ (find_max_pos l).
+
+Theorem freshness : forall s, ~In (fresh_ident s) s.
+Proof.
+  intros. unfold fresh_ident.
+  intro.
+  apply Lessthan in H.
+  assert (Plt (find_max_pos s) (Pos.succ (find_max_pos s))). apply Plt_succ.
+  assert (Plt (find_max_pos s) (find_max_pos s)). eapply Plt_Ple_trans. eauto. auto.
+  apply Plt_strict in H1.
+  auto.
+Qed.
+
+End Memstructure1.
+
+
