common/Values.v
@@ -29,13 +29,14 @@ Parameter eq_block : forall (x y:block),{x=y}+{x<>y}.
 
 End BLOCK.
 
-(* Declare Module Block : BLOCK. *)
+(* Declare Module Block : BLOCK.
 
 Module Block <: BLOCK.
 Definition block := positive.
 Definition eq_block := peq.
 End Block.
 
+*)
 (* NO GLOBAL INSTANCE
  Definition block := Block.block.
  Definition eq_block := Block.eq_block.
